examples/dev/sw/preARMSyntax.sml
@@ -10,9 +10,9 @@ in
 (*----------------------------------------------------------------------------*)
 
 fun eval_exp (Assem.MEM {reg = regNo, offset = offset, wback = flag}) =
-      mk_comb(Term`MEM:(num # num) -> EXP`, 
-              	mk_pair(term_of_int regNo, 
-	          mk_comb(if offset >= 0 then Term`POS` else Term`NEG`, 
+      mk_comb(Term`MEM:(num # num) -> EXP`,
+                mk_pair(term_of_int regNo,
+                  mk_comb(if offset >= 0 then Term`POS` else Term`NEG`,
                           term_of_int offset)))
  |  eval_exp (Assem.NCONST e) =
       mk_comb(Term`NCONST`, term_of_int e)
@@ -29,52 +29,56 @@ fun eval_exp (Assem.MEM {reg = regNo, offset = offset, wback = flag}) =
 
 fun mk_ARM arm =
   let
-    val (fname, ftype, args,stms,outs) = arm;
 
     fun mk_stm (Assem.OPER {oper = (op1, cond1, flag), dst = dlist, src = slist, jump = jumps}) =
-        let 
-	    val ops = list_mk_pair [mk_const(Assem.print_op op1, Type `:OPERATOR`),
-				     if cond1 = NONE then mk_none (Type `:COND`)
-				     else mk_comb(Term`SOME:COND->COND option`, mk_const(Assem.print_cond cond1, Type `:COND`)), 
-				     boolSyntax.F]
-            val j1 = case (List.find (fn e => e = Assem.REG 15 orelse e = Assem.WREG 15) dlist)	of  (* check whether the pc is in the destination list *)  
-			NONE => (case jumps of
-                         	       NONE => mk_none (Type `:OFFSET`)
-                      		    |  SOME l =>
-                                		if Symbol.name (hd l) = "+" then
-                                        		mk_some (mk_comb(Term`POS`, term_of_int (Symbol.index (hd l))))
-                                		else mk_some (mk_comb(Term`NEG`, term_of_int (Symbol.index (hd l))))
-                     		) |
-			SOME l => mk_some (Term`INR`)	(* the pc is modified to be the value in a register *)
+        let
+            val ops = list_mk_pair [mk_const(Assem.print_op op1, Type `:OPERATOR`),
+                                     if cond1 = NONE then mk_none (Type `:COND`)
+                                     else mk_comb(Term`SOME:COND->COND option`,
+                                                   mk_const(Assem.print_cond cond1, Type `:COND`)),
+                                     Term`F`]
 
-	    val (slist,dlist) = if op1 = Assem.LDMFD orelse op1 = Assem.STR then (dlist,slist)
-				else if op1 = Assem.CMP then (slist, [])
-				else (slist,dlist)
-	    val d1 = if length dlist = 0 then 
-			mk_none (Type `:EXP`)
-		     else mk_some (eval_exp (hd dlist));
+            val j1 = case (List.find (fn e => e = Assem.REG 15 orelse e = Assem.WREG 15) dlist) of
+                                (* check whether the pc is in the destination list *)
+                        NONE => (case jumps of
+                                       NONE => mk_none (Type `:OFFSET`)
+                                    |  SOME l =>
+                                                if Symbol.name (hd l) = "+" then
+                                                        mk_some (mk_comb(Term`POS`, term_of_int (Symbol.index (hd l))))
+                                                else mk_some (mk_comb(Term`NEG`, term_of_int (Symbol.index (hd l))))
+                                ) |
+                        SOME l => mk_some (Term`INR`)     (* the pc is modified to be the value in a register *)
+
+            val (slist,dlist) = if op1 = Assem.LDMFD orelse op1 = Assem.STR then (dlist,slist)
+                                else if op1 = Assem.CMP then (slist, [])
+                                else (slist,dlist)
+            val d1 = if length dlist = 0 then
+                        mk_none (Type `:EXP`)
+                     else mk_some (eval_exp (hd dlist));
             val s1 = mk_list (List.map eval_exp slist, Type `:EXP`);
+
         in
             list_mk_pair [ops,d1,s1,j1]
         end
 
-    |  mk_stm (Assem.MOVE inst) =
-        list_mk_pair [list_mk_pair [Term`MOV`, Term`NONE : COND option`, boolSyntax.F],
+   |  mk_stm (Assem.MOVE inst) =
+        list_mk_pair [list_mk_pair [Term`MOV`, Term`NONE : COND option`, Term`F`],
                       mk_some (eval_exp (#dst inst)),
                       mk_list ([eval_exp (#src inst)], Type `:EXP`),
                       mk_none (Type `:OFFSET`)
                      ]
 
     |  mk_stm (Assem.LABEL _) =
-	( print "Please use link2 to remove the labels first \n";
-	  raise ERR "ARM" ("invalid ARM program")
-	)
+        ( print "Please use link2 to remove the labels first \n";
+          raise ERR "ARM" ("invalid ARM program")
+        )
+
+    fun one_fun (fname, ftype, args, stms, outs, rs) =
+        List.map mk_stm stms;
 
   in
-     ( fname, ftype,
-       args,
-       mk_list(List.map mk_stm stms, Type `:INST`),
-       outs
+     (arm,
+      mk_list(List.foldl (fn (f,instL) => instL @ (one_fun f)) [] arm, Type `:INST`)
      )
   end
 
