examples/dev/sw/preARMScript.sml
@@ -1,23 +1,32 @@
-(*
-  quietdec := true;
-  app load ["word32Theory", "word32Lib", "whileTheory"];
-  open HolKernel Parse boolLib bossLib numLib
-       arithmeticTheory word32Theory pairTheory listTheory whileTheory;
-  quietdec := false;
-*)
-
 open HolKernel Parse boolLib bossLib numLib
      arithmeticTheory word32Theory pairTheory listTheory whileTheory;
 
 val _ = new_theory "preARM";
 
 (*----------------------------------------------------------------------------*)
-(* Registers and such                                                         *)
+(* Preprocessing                                                              *)
 (*----------------------------------------------------------------------------*)
 
-val _ = type_abbrev("REGISTER",``:num``);
-val _ = type_abbrev("ADDR", Type`:num`);
-val _ = type_abbrev("DATA", Type`:word32`);
+val _ = add_rule{term_name   = "COND",
+fixity      = Infix (HOLgrammars.RIGHT, 3),
+pp_elements = [HardSpace 1, TOK "=>", BreakSpace(1,0), TM, BreakSpace(1,0), TOK "|", HardSpace 1],
+paren_style = OnlyIfNecessary,
+block_style = (AroundEachPhrase, (PP.INCONSISTENT, 0))};
+
+(*
+val _ = add_rule{term_name   = "COND",
+fixity      = TruePrefix 70,
+pp_elements = [PPBlock([TOK "if", BreakSpace(1,2), TM, BreakSpace(1,0),TOK "then"], (CONSISTENT, 0)),
+	       BreakSpace(1,2), TM, BreakSpace(1,0), TOK "else", BreakSpace(1,2)],
+paren_style = Always,
+block_style = (AroundEachPhrase, (PP.CONSISTENT, 0))};
+*)
+
+(*----------------------------------------------------------------------------*)
+(* Registers	                                                              *)
+(*----------------------------------------------------------------------------*)
+
+val _ = type_abbrev("REGISTER", Type`:num`);
 
 (*----------------------------------------------------------------------------*)
 (* CPSR, In user programs only the top 4 bits of the CPSR are relevant        *)
@@ -28,10 +37,9 @@ val _ = type_abbrev("DATA", Type`:word32`);
 (*----------------------------------------------------------------------------*)
 
 val _ = type_abbrev("CPSR", Type`:word32`);
-
 val _ = Hol_datatype `SRS = SN | SZ | SC | SV`;
 
-val getS = Define
+val getS_def = Define
         `getS (cpsr : CPSR) (flag:SRS) =
             case flag of
                  SN -> MSB cpsr ||
@@ -40,7 +48,16 @@ val getS = Define
                  SV -> MSB (cpsr << 3)
         `;
 
-val setS = Define
+val getS_thm = Q.prove (
+        `(getS (cpsr : CPSR) SN = MSB cpsr) /\ 
+	 (getS (cpsr : CPSR) SZ = MSB (cpsr << 1)) /\
+	 (getS (cpsr : CPSR) SC = MSB (cpsr << 2)) /\
+	 (getS (cpsr : CPSR) SV = MSB (cpsr << 3))
+	`,
+	RW_TAC std_ss [getS_def]);
+
+
+val setS_def = Define
         `setS (cpsr : CPSR) (flag:SRS) =
             case flag of
                  SN -> (cpsr | 0x80000000w) ||
@@ -48,6 +65,15 @@ val setS = Define
                  SC -> (cpsr | 0x20000000w) ||
                  SV -> (cpsr | 0x10000000w)
         `;
+
+val setS_thm = Q.prove (
+        `(setS (cpsr : CPSR) SN = (cpsr | 0x80000000w)) /\
+	 (setS (cpsr : CPSR) SZ = (cpsr | 0x40000000w)) /\
+	 (setS (cpsr : CPSR) SC = (cpsr | 0x20000000w)) /\
+	 (setS (cpsr : CPSR) SV = (cpsr | 0x10000000w))
+        `,
+	RW_TAC std_ss [setS_def]);
+
 
 (*-------------------------------------------------------------------------------*)
 (* Operator			                                                 *)
@@ -60,8 +86,7 @@ val _ = Hol_datatype ` OPERATOR = MOV |
                         LDR | STR | LDMFD | STMFD |
                         MRS | MSR |
                         B | BL |
-                        SWI | DCD |
-                        NOP
+                        SWI
              `;
 
 val OPERATOR_cases = TypeBase.nchotomy_of "OPERATOR";
@@ -79,35 +104,30 @@ val COND_cases = TypeBase.nchotomy_of "COND";
 (* Expressions			                                                 *)
 (*-------------------------------------------------------------------------------*)
 
-val _ = 
- Hol_datatype `OFFSET = POS of ADDR
+val _ = type_abbrev("ADDR", Type`:num`);
+
+val _ = Hol_datatype `OFFSET = POS of ADDR
                | NEG of ADDR
 	       | INR
              `;
 
 
-val _ = 
- Hol_datatype `EXP = MEM of num # OFFSET	(* (register, offset) *) 
+val _ = Hol_datatype `EXP = MEM of num # OFFSET			(* (register, offset) *) 
                   | NCONST of num
 		  | WCONST of word32
                   | REG of REGISTER
 		  | WREG of REGISTER
              `;
 
-val _ = type_abbrev("ADDR", Type`:num`);
 val _ = type_abbrev("DATA", Type`:word32`);
-
 
 (*-------------------------------------------------------------------------------*)
 (* Operations                                                                    *)
 (*-------------------------------------------------------------------------------*)
 
 (* An operation: (operator, condition code, set flags, destination, source, jump)					 *)
-
-val _ = type_abbrev("OPERATION", ``:OPERATOR # (COND option) # bool``);
-
-val _ = type_abbrev("INST", 
-            ``:OPERATION # (EXP option) # (EXP list) # (OFFSET option)``);
+val _ = type_abbrev("OPERATION", Type`:OPERATOR # (COND option) # bool`);
+val _ = type_abbrev("INST", Type`:OPERATION # (EXP option) # (EXP list) # (OFFSET option)`);
 
 (*---------------------------------------------------------------------------------*)
 (* Memory	                                                                   *)
@@ -115,15 +135,17 @@ val _ = type_abbrev("INST",
 
 (* store to the instruction buffer or the data buffer (both in the memory)	   *)               
 val STORE_def =
- Define 
-   `STORE (mem:ADDR->'a) addr v = \k. if k = addr then v else mem k
-   `;
+  Define `
+     STORE (mem:ADDR->'a) addr v =
+        \k. if k = addr then v
+            else mem k
+  `;
 
 (*---------------------------------------------------------------------------------*)
 (* State                                                                           *)
 (*---------------------------------------------------------------------------------*)
   
-val _ = type_abbrev("STATE", ``: ADDR # CPSR # (REGISTER -> DATA) # (ADDR -> DATA)``);
+val _ = type_abbrev("STATE", Type`: ADDR # CPSR # (REGISTER -> DATA) # (ADDR -> DATA)`);
 
 val FORALL_STATUS = Q.store_thm
   ("FORALL_STATUS",
@@ -136,14 +158,13 @@ val FORALL_STATE = Q.store_thm
     `(!s:STATE. P s) = !pc pcsr regs mem. P (pc,pcsr,(regs,mem))`,
     SIMP_TAC std_ss [FORALL_PROD]);  
                
-
 (*---------------------------------------------------------------------------------*)
 (* Read and write registers and memory                                             *)
 (*---------------------------------------------------------------------------------*)
 
 val read_def =
- Define 
-   `read ((regs,mem):(ADDR->DATA)#(ADDR->DATA)) (exp:EXP) =
+  Define `
+    read ((regs,mem):(ADDR->DATA)#(ADDR->DATA)) (exp:EXP) =
       case exp of
         MEM (r,offset) -> 
 	    (case offset of 
@@ -154,10 +175,19 @@ val read_def =
         WCONST w -> w         ||
         REG r -> regs r
   `;
+
+val read_thm = Q.prove (
+  ` (read (regs,mem) (MEM (r,POS k)) = mem (w2n (regs r) + k)) /\
+    (read (regs,mem) (MEM (r,NEG k)) = mem (w2n (regs r) - k)) /\
+    (read (regs,mem) (NCONST i) = n2w i) /\
+    (read (regs,mem) (WCONST w) = w) /\
+    (read (regs,mem) (REG r) = regs r)`,
+    RW_TAC std_ss [read_def]);
+
             
 val write_def =
- Define 
-   `write ((regs,mem):(ADDR->DATA)#(ADDR->DATA)) (exp:EXP) (v:DATA)=
+  Define `
+    write ((regs,mem):(ADDR->DATA)#(ADDR->DATA)) (exp:EXP) (v:DATA)=
       case exp of
         MEM (r,offset) -> 
 	    (regs,
@@ -170,10 +200,19 @@ val write_def =
                    mem ) ||
         _ -> (regs, mem)
   `;
-                      
+
+val write_thm = Q.prove (
+  ` (write (regs,mem) (MEM (r,POS k)) v = (regs, (\addr. if addr = w2n (regs r) + k then v
+            				      	      else mem addr))) /\
+    (write (regs,mem) (MEM (r,NEG k)) v = (regs, (\addr. if addr = w2n (regs r) - k then v
+                                                      else mem addr))) /\
+    (write (regs,mem) (REG r) v = ((\k. if k = r then v
+                        		else regs k),
+                   		   mem ))`,
+    RW_TAC std_ss [write_def, STORE_def]);                      
 
 (*---------------------------------------------------------------------------------*)
-(* Decoding                                                                        *)
+(* Decoding and execution of an instruction                                        *)
 (*---------------------------------------------------------------------------------*)
 
 val goto_def =
@@ -185,13 +224,24 @@ val goto_def =
 	    INR ->   pc
    `;
 
-val read_pc_def = 
-  Define `
-    read_pc (cpsr,s) = (w2n (read s (REG 15)), cpsr, s)`;
+val goto_thm = Q.prove (
+  ` (goto (pc, SOME (POS n)) = pc + n) /\
+    (goto (pc, SOME (NEG n)) = pc - n) /\
+    (goto (pc, SOME INR) = pc)
+  `,
+  RW_TAC std_ss [goto_def]);
 
-val set_pc_def =
+
+val read_pc = 
   Define `
-    set_pc s pc = (pc, FST s, write (SND s) (REG 15) (n2w pc))`;
+    read_pc (cpsr,s) = 
+		(w2n (read s (REG 15)), cpsr, s)`;
+
+val set_pc =
+  Define `
+    set_pc s pc =
+                (pc, FST s, write (SND s) (REG 15) (n2w pc))`;
+
 
 val decode1_def = 
   Define `
@@ -283,6 +333,64 @@ val decode1_def =
           _  ->  ARB
   `;
 
+val decode1_thm = Q.prove
+(`!pc cpsr s dst src jump.
+  (decode1 (pc,cpsr,s) (MOV,SOME dst,src,jump) = (cpsr, write s dst (read s (HD src)))) /\
+  (decode1 (pc,cpsr,s) (ADD,SOME dst,src,jump) = (cpsr, write s dst (read s (HD src) + read s (HD (TL src))))) /\
+  (decode1 (pc,cpsr,s) (SUB,SOME dst,src,jump) = (cpsr, write s dst (read s (HD src) - read s (HD (TL src))))) /\
+  (decode1 (pc,cpsr,s) (RSB,SOME dst,src,jump) = (cpsr, write s dst (read s (HD (TL src)) - read s (HD src)))) /\
+  (decode1 (pc,cpsr,s) (MUL,SOME dst,src,jump) = (cpsr, write s dst (read s (HD src) * read s (HD (TL src))))) /\
+  (decode1 (pc,cpsr,s) (MLA,SOME dst,src,jump) = (cpsr, write s dst (read s (HD src) * read s (HD (TL src)) + read s (HD (TL (TL src)))))) /\
+  (decode1 (pc,cpsr,s) (AND,SOME dst,src,jump) = (cpsr, write s dst (read s (HD src) & read s (HD (TL src))))) /\
+  (decode1 (pc,cpsr,s) (ORR,SOME dst,src,jump) = (cpsr, write s dst (read s (HD src) | read s (HD (TL src))))) /\
+  (decode1 (pc,cpsr,s) (EOR,SOME dst,src,jump) = (cpsr, write s dst (read s (HD src) # read s (HD (TL src))))) /\
+  (decode1 (pc,cpsr,s) (CMP,NONE,src,jump) = (if read s (HD src) = read s (HD (TL src))
+                                             then (setS 0w SZ,s)
+                                             else (if read s (HD src) < read s (HD (TL src))
+                                                   then (setS 0w SN,s)
+                                                   else (setS 0w SC,s)))) /\
+  (decode1 (pc,cpsr,s) (TST,NONE,src,jump) = (if read s (HD src) & read s (HD (TL src)) = 0w
+                                             then (setS cpsr SZ,s) else (cpsr,s))) /\
+  (decode1 (pc,cpsr,s) (LSL,SOME dst,src,jump) = (cpsr, write s dst (read s (HD src) << w2n (read s (HD (TL src)))))) /\
+  (decode1 (pc,cpsr,s) (LSR,SOME dst,src,jump) = (cpsr, write s dst (read s (HD src) >>> w2n (read s (HD (TL src)))))) /\
+  (decode1 (pc,cpsr,s) (ASR,SOME dst,src,jump) = (cpsr, write s dst (read s (HD src) >> w2n (read s (HD (TL src)))))) /\
+  (decode1 (pc,cpsr,s) (ROR,SOME dst,src,jump) = (cpsr, write s dst (read s (HD src) #>> w2n (read s (HD (TL src)))))) /\
+  (decode1 (pc,cpsr,s) (LDR,SOME dst,src,jump) = (cpsr, write s dst (read s (HD src)))) /\
+  (decode1 (pc,cpsr,s) (STR,SOME dst,src,jump) = (cpsr, write s (HD src) (read s dst))) /\
+  (decode1 (pc,cpsr,s) (LDMFD, SOME (REG r),src,jump) =
+              (cpsr, FST (FOLDL
+                          (\(s,i) reg.
+                             (write s reg (read s (MEM (r,POS (i + 1)))),
+                              i + 1)) (s,0) src))) /\
+  (decode1 (pc,cpsr,s) (LDMFD,SOME (WREG r),src,jump) =
+              (cpsr, write (FST
+                             (FOLDL
+                               (\(s,i) reg.
+                                (write s reg
+                                   (read s (MEM (r,POS (i + 1)))),i + 1))
+                               (s,0) src)) (REG r)
+                       	     (read s (REG r) + n2w (LENGTH src)))) /\
+  (decode1 (pc,cpsr,s) (STMFD,SOME (REG r),src,jump) =
+                  (cpsr, FST (FOLDL
+                          (\(s,i) reg.
+                             (write s (MEM (r,NEG i)) (read s reg),i + 1))
+                          (s,0) (REVERSE src)))) /\
+  (decode1 (pc,cpsr,s) (STMFD,SOME (WREG r),src,jump) =
+                  (cpsr, write (FST
+                          (FOLDL
+                             (\(s,i) reg.
+                                (write s (MEM (r,NEG i)) (read s reg),
+                                 i + 1)) (s,0) (REVERSE src))) (REG r)
+                       (read s (REG r) - n2w (LENGTH src)))) /\
+  (decode1 (pc,cpsr,s) (MRS,SOME dst,src,jump) = (cpsr,write s dst cpsr)) /\
+  (decode1 (pc,cpsr,s) (MSR,NONE,src,jump) = (read s (HD src),s)) /\
+  (decode1 (pc,cpsr,s) (B,NONE,src,jump) = (cpsr,write s (REG 15) (n2w (goto (pc,jump))))) /\
+  (decode1 (pc,cpsr,s) (BL,NONE,src,jump) = (cpsr,write (write s (REG 14) (word_suc (n2w pc))) (REG 15)
+                                                    (n2w (goto (pc,jump)))))`,
+ 
+   RW_TAC std_ss [decode1_def]);
+  
+
   
 val decode2_def =
   Define `
@@ -316,6 +424,44 @@ val decode2_def =
 		)
   `;
 
+val decode2_thm = Q.prove
+(`!pc cpsr s op sflag dst src jump.
+  (decode2 (pc,cpsr,s) ((op,NONE,sflag),dst,src,jump) = set_pc (decode1 (pc,cpsr,s) (op,dst,src,jump)) (pc + 1)) /\
+  (decode2 (pc,cpsr,s) ((op,SOME EQ,sflag),dst,src,jump) =
+              (if getS cpsr SZ then
+                 read_pc (decode1 (pc,cpsr,s) (op,dst,src,jump))
+               else
+                 (pc + 1,cpsr,write s (REG 15) (n2w (pc + 1))))) /\
+  (decode2 (pc,cpsr,s) ((op,SOME NE,sflag),dst,src,jump) =
+              (if getS cpsr SZ then
+                 (pc + 1,cpsr,write s (REG 15) (n2w (pc + 1)))
+               else
+                 read_pc (decode1 (pc,cpsr,s) (op,dst,src,jump)))) /\
+  (decode2 (pc,cpsr,s) ((op,SOME GE,sflag),dst,src,jump) =
+              (if getS cpsr SN then
+                 (pc + 1,cpsr,write s (REG 15) (n2w (pc + 1)))
+               else
+                 read_pc (decode1 (pc,cpsr,s) (op,dst,src,jump)))) /\
+  (decode2 (pc,cpsr,s) ((op,SOME LE,sflag),dst,src,jump) =
+              (if getS cpsr SC then
+                 (pc + 1,cpsr,write s (REG 15) (n2w (pc + 1)))
+               else
+                 read_pc (decode1 (pc,cpsr,s) (op,dst,src,jump)))) /\
+  (decode2 (pc,cpsr,s) ((op,SOME GT,sflag),dst,src,jump) =
+              (if getS cpsr SC then
+                 read_pc (decode1 (pc,cpsr,s) (op,dst,src,jump))
+               else
+                 (pc + 1,cpsr,write s (REG 15) (n2w (pc + 1))))) /\
+  (decode2 (pc,cpsr,s) ((op,SOME LT,sflag),dst,src,jump) =
+              (if getS cpsr SN then
+                 read_pc (decode1 (pc,cpsr,s) (op,dst,src,jump))
+               else
+                 (pc + 1,cpsr,write s (REG 15) (n2w (pc + 1))))) /\
+  (decode2 (pc,cpsr,s) ((op,SOME AL,sflag),dst,src,jump) = read_pc (decode1 (pc,cpsr,s) (op,dst,src,jump))) /\
+  (decode2 (pc,cpsr,s) ((op,SOME NV,sflag),dst,src,jump) = (pc + 1,cpsr,write s (REG 15) (n2w (pc + 1))))`,
+  RW_TAC std_ss [decode2_def]);
+
+
 (*---------------------------------------------------------------------------------*)
 (* Upload instructions into the instruction buffer                                 *)
 (*---------------------------------------------------------------------------------*)
@@ -325,13 +471,13 @@ val decode2_def =
                                      
 val upload_def =
   Define `  
-    (upload (stm::rest) instB start =
+    (upload (stm::rest) iB start =
         \addr. if addr = start then stm
-               else (upload rest instB (SUC start)) addr) /\
-    (upload [] instB start = instB)
+               else (upload rest iB (SUC start)) addr) /\
+    (upload ([]) iB start = iB)
   `;
                 
-val UPLOAD_LEM = Q.store_thm ("UPLOAD_LEM",
+val UPLOAD_LEM = Q.prove (
   `!instL start instB addr. addr < LENGTH instL ==>
 	((upload instL instB start) (start+addr) = (upload instL instB 0) addr)`,
   Induct_on `addr` THEN Induct_on `instL` THEN RW_TAC list_ss [upload_def] THEN
@@ -341,11 +487,10 @@ val UPLOAD_LEM = Q.store_thm ("UPLOAD_LEM",
 
             
 val uploadCode_def =
-  Define 
-   `uploadCode instL instB = upload instL instB 0`;
+  Define `uploadCode instL iB = upload instL iB 0`;
 
                                      
-val UPLOADCODE_LEM = Q.store_thm ("UPLOADCODE_LEM",
+val UPLOADCODE_LEM = Q.prove (
    `!instL instB n. n < LENGTH instL ==>
         ((uploadCode instL instB) n = EL n instL)`,
     SIMP_TAC list_ss [uploadCode_def] THEN Induct_on `n` THEN
@@ -353,25 +498,20 @@ val UPLOADCODE_LEM = Q.store_thm ("UPLOADCODE_LEM",
     METIS_TAC [SUC_ONE_ADD, UPLOAD_LEM, ADD_SYM]
    );
         
-val UPLOAD_THM = Q.store_thm ("UPLOAD_THM",
+val UPLOAD_THM = Q.prove (
    `!instL instB n. n < LENGTH instL ==>
         ((upload instL instB start) (start+n) = EL n instL)`,
     METIS_TAC [uploadCode_def, UPLOAD_LEM, UPLOADCODE_LEM ]
    );
 
-
 val uploadSeg_def = Define `
-    (uploadSeg 0 segs instB = instB) /\
-    (uploadSeg (SUC n) segs instB = 
-	upload (EL n segs) (uploadSeg n segs instB) (10 * n))`;
+    (uploadSeg 0 segs iB = iB) /\
+    (uploadSeg (SUC n) segs iB = 
+	upload (EL n segs) (uploadSeg n segs iB) (10 * n))`;
 
-val UPLOADSEG_LEM = Q.store_thm
-  ("UPLOADSEG_LEM",
-   `!n segs instB. uploadSeg n segs instB = 
-	if n > 0 
-          then upload (EL (PRE n) segs) 
-                      (uploadSeg (PRE n) segs instB) (10 * (PRE n)) 
-          else instB`,
+val UPLOADSEG_LEM = Q.prove
+  (`!n segs instB. uploadSeg n segs instB = 
+	(if n > 0 then upload (EL (PRE n) segs) (uploadSeg (PRE n) segs instB) (10 * (PRE n)) else instB)`,
     Cases_on `n` THEN RW_TAC list_ss [uploadSeg_def]
   );
 
@@ -379,23 +519,21 @@ val UPLOADSEG_LEM = Q.store_thm
 (* Running of a ARM program                                                        *)
 (*---------------------------------------------------------------------------------*)
 
-val (run_def,run_ind) = 
- Defn.tprove
-  (Hol_defn "run"
-    `run n (instB,byn) (pc,cpsr,st) = 
+val (run_def,run_ind)  =
+  Defn.tprove (
+  Defn.Hol_defn "run" `
+      run n (iB,byn) (pc,cpsr,st) = 
 	if n = 0 then (pc,cpsr,st)
 	else 
       	    if pc = byn then (pc,cpsr,st) 
       	    else
-		run (n-1) (instB,byn) (decode2 (pc,cpsr,st) (instB pc))`,
-    WF_REL_TAC `measure FST`);
+		run (n-1) (iB,byn) (decode2 (pc,cpsr,st) (iB pc)) 
+  `,
+  WF_REL_TAC `measure FST`
+  );
 
-val _ = save_thm("run_def", run_def);
-val _ = save_thm("run_ind", run_ind);
-
-val RUN_LEM_1 = Q.store_thm
-  ("RUN_LEM_1",
-   `!n instB byn s.
+val RUN_LEM_1 = Q.prove
+  (`!n instB byn s.
         (run (SUC n) (instB,byn) s = 
 		if FST s = byn then s 
 		else run n (instB,byn) (decode2 s (instB (FST s)))
@@ -410,17 +548,15 @@ val RUN_LEM_1 = Q.store_thm
    	ONCE_ASM_REWRITE_TAC [] THEN RW_TAC list_ss []]
   );
 
-val RUN_LEM_2 = Q.store_thm
-  ("RUN_LEM_2",
-   `!n instB s. run n (instB,FST s) s = s`,
+val RUN_LEM_2 = Q.prove
+  (`!n instB s. run n (instB,FST s) s = s`,
    SIMP_TAC list_ss [FORALL_STATE] THEN
    Induct_on `n` THEN RW_TAC list_ss [RUN_LEM_1]
   );
 
 
-val RUN_THM_1 = Q.store_thm
-  ("RUN_THM_1",
-   `!m n s instB byn.
+val RUN_THM_1 = Q.prove
+  (`!m n s instB byn.
         (run (m+n) (instB,byn) s = run n (instB,byn) (run m (instB,byn) s))`,
   Induct_on `m` THEN REPEAT GEN_TAC THENL [
         RW_TAC list_ss [RUN_LEM_1],
@@ -429,19 +565,42 @@ val RUN_THM_1 = Q.store_thm
         RW_TAC list_ss [RUN_LEM_2]]
   );
 
-val RUN_THM_2 = Q.store_thm
-  ("RUN_THM_2",
-   `!m n s instB byn. m <= n ==>
+val RUN_THM_2 = Q.prove
+  (`!m n s instB byn. m <= n ==>
         (run n (instB,byn) s = run (n-m) (instB,byn) (run m (instB,byn) s))`,
   RW_TAC list_ss [] THEN `?k. n = k + m` by PROVE_TAC [LESS_EQUAL_ADD, ADD_SYM] THEN 
   ASM_REWRITE_TAC [] THEN METIS_TAC [SUB_ADD, RUN_THM_1, ADD_SYM]
   );
 
+(*---------------------------------------------------------------------------------*)
+(* Run to termination                                                              *)
+(*---------------------------------------------------------------------------------*)
+
+fun LEAST_ELIM_TAC (asl, w) = 
+  let
+    val least_terms = find_terms numSyntax.is_least w
+    val tbc = TRY_CONV BETA_CONV
+    fun doit t =
+    if free_in t w then
+    CONV_TAC (UNBETA_CONV t) THEN
+    MATCH_MP_TAC whileTheory.LEAST_ELIM THEN
+    CONV_TAC
+    (FORK_CONV
+    (BINDER_CONV tbc, (* ?n. P n *)
+            BINDER_CONV      (* !n. (!m. m < n ==> ~P m) /\ P n ==> Q n *)
+    (FORK_CONV
+    (FORK_CONV
+                    (BINDER_CONV (RAND_CONV (RAND_CONV tbc)), (* !m.... *)
+	tbc), (* P n *)
+               tbc))))
+    	else NO_TAC
+  in
+    FIRST (map doit least_terms)
+  end (asl, w);
 
 val _ = Globals.priming := NONE;
 
-val LEAST_ADD_LEM = Q.store_thm 
- ("LEAST_ADD_LEM",
+val LEAST_ADD_LEM = Q.prove (
   `!P m. (?n. P n) /\ m <= (LEAST n. P n) ==>
            ((LEAST n. P n) = (LEAST n. P (m + n)) + m)`,
   Induct_on `m` THENL [
@@ -465,14 +624,13 @@ val LEAST_ADD_LEM = Q.store_thm
 (* n is the maximum numbers for all paths of the program to terminate                                                           *)
 
 val terminated_def =
- Define 
-   `terminated (instB,byn) s = ?n. FST (run n (instB,byn) s) = byn`;
+  Define `!instB byn s. terminated (instB,byn) s = 
+	?n. (FST (run n (instB,byn) s) = byn)`;
 
 
-val TERMINATED_THM = Q.store_thm
-  ("TERMINATED_THM",
-   `!m s iB byn n. 
-       terminated (iB,byn) s ==> terminated (iB,byn) (run m (iB,byn) s)`,
+val TERMINATED_THM = Q.prove
+  (`!m s iB byn n. (terminated (iB,byn) s) ==>
+        (terminated (iB,byn) (run m (iB,byn) s))`,
   RW_TAC list_ss [terminated_def, GSYM RUN_THM_1] THEN
   ONCE_REWRITE_TAC [ADD_SYM] THEN 
   RW_TAC list_ss [RUN_THM_1] THEN
@@ -482,15 +640,13 @@ val TERMINATED_THM = Q.store_thm
 
 
 val minStep_def =  
-  Define `minStep (instB,byn) s = LEAST n. FST (run n (instB,byn) s) = byn`;
+  Define `!instB byn s. minStep (instB,byn) s = 
+	$LEAST (\n. FST (run n (instB,byn) s) = byn)`;
 
 
-val MINSTEP_THM = Q.store_thm
-  ("MIN_STEP_THM",
-   `!s instB byn m. 
-       (terminated (instB,byn) s) /\ 
-       (m <= minStep (instB,byn) s) ==>
-       (minStep (instB,byn) s = (minStep (instB,byn) (run m (instB,byn) s) + m))`,
+val MINSTEP_THM = Q.prove
+  (`!s instB byn m. (terminated (instB,byn) s) /\ (m <= minStep (instB,byn) s) ==>
+        (minStep (instB,byn) s = (minStep (instB,byn) (run m (instB,byn) s) + m))`,
     RW_TAC list_ss [terminated_def, minStep_def] THEN
     RW_TAC list_ss [ONCE_REWRITE_RULE [EQ_SYM_EQ] RUN_THM_1] THEN 
     ONCE_REWRITE_TAC [ADD_SYM] THEN
@@ -500,12 +656,11 @@ val MINSTEP_THM = Q.store_thm
 
 
 val terRun_def = 
-  Define 
-   `terRun (instB,byn) s = run (minStep (instB,byn) s) (instB,byn) s`; 
+  Define `!instB byn s. terRun (instB,byn) s = 
+	run (minStep (instB,byn) s) (instB,byn) s`; 
 
-val TERRUN_LEM_1 = Q.store_thm
-  ("TERRUN_LEM_1",
-   `!s iB byn. (terminated (iB,byn) s) ==>
+val TERRUN_LEM_1 = Q.prove
+  (`!s iB byn. (terminated (iB,byn) s) ==>
         (terRun (iB,byn) (terRun (iB,byn) s) = terRun (iB,byn) s)`,
     RW_TAC list_ss [terRun_def, minStep_def, terminated_def] THEN
     LEAST_ELIM_TAC THEN RW_TAC list_ss [] THENL [
@@ -515,9 +670,8 @@ val TERRUN_LEM_1 = Q.store_thm
    );
 
 
-val TERRUN_LEM_2 = Q.store_thm
-  ("TERRUN_LEM_2",
-   `!s iB byn m. (terminated (iB,byn) s /\ m > minStep (iB,byn) s) ==>
+val TERRUN_LEM_2 = Q.prove
+  (`!s iB byn m. (terminated (iB,byn) s /\ m > minStep (iB,byn) s) ==>
         (terRun (iB,byn) s = run m (iB,byn) s)`,
     RW_TAC list_ss [terRun_def, terminated_def] THEN
     `?k. m = minStep (iB,byn) s + k` by METIS_TAC [GREATER_DEF, LESS_EQ_EXISTS, LESS_IMP_LESS_OR_EQ, ADD_SYM]
@@ -529,9 +683,8 @@ val TERRUN_LEM_2 = Q.store_thm
         ]
    );
 
-val TERRUN_THM = Q.store_thm
-  ("TERRUN_THM",
-   `!m s iB byn n. (terminated (iB,byn) s) ==> 
+val TERRUN_THM = Q.prove
+  (`!m s iB byn n. (terminated (iB,byn) s) ==> 
         (terRun (iB,byn) s = terRun (iB,byn) (run m (iB,byn) s))`,
   REPEAT STRIP_TAC THEN
   Cases_on `m <= minStep (iB,byn) s` THENL [
@@ -540,18 +693,16 @@ val TERRUN_THM = Q.store_thm
      METIS_TAC [NOT_LESS_EQUAL, GREATER_DEF, TERRUN_LEM_2, TERRUN_LEM_1]]
   );
 
-val TERMINATED_EXPAND_1 = Q.store_thm
-  ("TERMINATED_EXPAND_1",
-   `!s iB byn. terminated (iB,byn) s ==> (FST s) < byn ==> 
+val TERMINATED_EXPAND_1 = Q.prove
+  (`!s iB byn. terminated (iB,byn) s ==> (FST s) < byn ==> 
         terminated (iB,byn) (decode2 s (iB (FST s)))`,
   RW_TAC list_ss [terminated_def] THEN
   Cases_on `n` THEN FULL_SIMP_TAC list_ss [RUN_LEM_1] THEN
   METIS_TAC []
   );
 
-val TERRUN_EXPAND_1 = Q.store_thm
-  ("TERRUN_EXPAND_1",
-   `!s iB byn. terminated (iB,byn) s ==> (FST s) < byn ==>  
+val TERRUN_EXPAND_1 = Q.prove
+  (`!s iB byn. terminated (iB,byn) s ==> (FST s) < byn ==>  
         (terRun (iB,byn) s = terRun (iB,byn) (decode2 s (iB (FST s))))`,
   RW_TAC list_ss [] THEN ASSUME_TAC (Q.SPEC `1` TERRUN_THM) THEN 	
   RES_TAC THEN 
@@ -561,9 +712,8 @@ val TERRUN_EXPAND_1 = Q.store_thm
   );
 
 
-val TERRUN_STOP = Q.store_thm
-  ("TERRUN_STOP",
-   `!s iB byn. (FST s = byn) ==>
+val TERRUN_STOP = Q.prove
+  (`!s iB byn. (FST s = byn) ==>
         (terRun (iB,byn) s = s)`,
   RW_TAC list_ss [terRun_def] THEN 
   RW_TAC list_ss [RUN_LEM_2]
@@ -571,38 +721,8 @@ val TERRUN_STOP = Q.store_thm
 
 
 (*---------------------------------------------------------------------------------*)
-(* Find the minStep for a given program                                            *)
-(*---------------------------------------------------------------------------------*)
-(*
-fun compute_minStep arm =
-  let
-    val (fname, ftype, args, stms, outs) = arm;
-
-    fun decode (Assem.OPER inst) pc =
-        	(case #jump inst of
-                         NONE => pc + 1
-                      |  SOME lab =>
-                                if Symbol.name (hd lab) = "+" then
-                                        pc + Symbol.index (hd lab)
-                                else pc - Symbol.index (hd lab)
-                     )
-    |  decode (Assem.MOVE inst) =
-		pc + 1
-    |  decode _ = raise ERR "ARM" ("invalid statement")
-
-    fun calulate stms = 
-	
-
-  in
-    
-  end
-*)
-	
-(*---------------------------------------------------------------------------------*)
 (* Recursion and loops	                                                           *)
 (*---------------------------------------------------------------------------------*)
-
-
 
 (* one entry and one exit													*)
 (* The following high-level definition says that if the running of L1 doesn't go beyond its range (never execute L2's), 	*)
@@ -615,7 +735,7 @@ fun compute_minStep arm =
 
 (* Theorem of Sequential Composition                                      			                                  *)
 (*
-val RUN_LEM_1 = Q.store_thm ("RUN_LEM_1",
+val RUN_LEM_1 = Q.prove (
     `!blk m start status.
 	(FST (runL m blk (start,status)) + start = FST (run m (upload blk start) (start,status))) /\
 	(SND (runL m blk (start,status)) = SND (run m (upload blk start) (start,status)))`,
@@ -629,7 +749,7 @@ val RUN_LEM_1 = Q.store_thm ("RUN_LEM_1",
 	RW_TAC list_ss [runL_def, run_def],
 
 
-val SEQ_COMP = Q.store_thm ("SEQ_COMP",
+val SEQ_COMP = Q.prove (
     `!blk1 blk2 m1 m2 s. e1e1 m1 blk1 s ==>
         (SND (runL m2 blk2 (runL m1 blk1 s)) = SND (runL (m1+m2) (blk1 ++ blk2) s))`,
     SIMP_TAC std_ss [FORALL_STATE] THEN Induct_on `m2` THENL [
@@ -638,7 +758,7 @@ val SEQ_COMP = Q.store_thm ("SEQ_COMP",
   );
 
    
-val COND_COMP = Q.store_thm (
+val COND_COMP = Q.prove (
     `(terminate cond /\ terminate tblk /\ terminate fblk) ==>
         !s. ?m1 m2 m3. runL m3 (cond ++ tblk ++ fblk) s =
                 let c = runL m0 cond s in
@@ -646,19 +766,13 @@ val COND_COMP = Q.store_thm (
                 else runL m2 fblk c`,
 *)
 
-(*---------------------------------------------------------------------------------*)
-(* Simulate ARM codes as functions                                                 *)
-(*---------------------------------------------------------------------------------*)
-
-val EL_THM = Q.store_thm
-  ("EL_THM",
-   `!n:num. EL n (h::t) = (if n > 0 then EL (PRE n) t else h)`,
+val EL_THM = Q.prove
+  (`!n:num. EL n (h::t) = (if n > 0 then EL (PRE n) t else h)`,
     Cases_on `n` THEN RW_TAC list_ss [EL]
   );
 
 (*---------------------------------------------------------------------------------*)
 (* Bisimulation. Compare source codes and  ARM codes synchronously                 *)
 (*---------------------------------------------------------------------------------*)
-
 
 val _ = export_theory();
