examples/dev/sw/examples/examples.sml
@@ -1,31 +1,8 @@
-(* For interactive work *)
- loadPath := "cps/" :: !loadPath;
-
-  quietdec := true;
-  app load ["word32Theory","ANF"];
-  open word32Theory pairTheory arithmeticTheory ANF;
-  quietdec := false;
+use "compiler";
 
 (*---------------------------------------------------------------------------*)
 (* Addition 	                                                             *)
 (*---------------------------------------------------------------------------*)
-
-val test0_def = Define
-  `test0 (t1:word32,t2:word32,t3:word32,t4:word32,t5:word32,t6:word32) =
-            (let k1 = UNCURRY $+ (t1,t5) in
-             let k2 = UNCURRY $- (k1, t6) in
-                (k1,k2,t5,t6)
-            )
-    `;
-
-
-val test0a_def = Define
-  `test0a (t1,t2) =
-            (let (k1,k2,k3,k4) = test0 (t1,t2,t1,t2,t1,t2) in
-                (k1,k2)
-            )
-    `;
-
 
 val test1_def = Define
   `test1 (t1:word32,t2:word32) =
@@ -56,19 +33,23 @@ val test3_def = Define
 
 (*
     val arm1 = link2 test1_def;
-    printarm arm1;
-    val ARM1 = mk_ARM arm1;
 
-        simT ARM1;
+Arguments:
+    r0 r1
+Body:
+    0:          mov     ip, sp
+    1:          stmfd   sp!, {fp,ip,lr,pc}
+    2:          sub     fp, ip, #1
+    3:          add     r2, r0, r1
+    4:          sub     r0, r0, r1
+    5:          sub     sp, fp, #2
+    6:          ldmfd   sp, {fp,sp,pc}
+Return:
+    r2 r0 
 
-    TAC0 [] THEN
-    REPEAT STRIP_TAC THEN 
-    IMP_RES_TAC (Q.SPEC `3` TERRUN_THM) THEN 	(* could be any number larger than 3 *)
-    ONCE_ASM_REWRITE_TAC [] THEN    
-    POP_ASSUM (K ALL_TAC) THEN
-    NTAC 3 TAC1 THEN
-    RW_TAC list_ss [TERRUN_STOP, test1_def,run_def]
-    
+    simT (mk_ARM arm1);
+
+    prove_arm [test1_def];
 
 *)
 
@@ -83,85 +64,68 @@ val (f6_def, f6_ind) = Defn.tprove
   WF_REL_TAC `measure (w2n o FST)` THEN METIS_TAC [WORD_PRED_THM] );
 
 (*
-Name: f6
 Arguments:
-    R3 R1
+    r0 r1
 Body:
-    0:        MOV R0, 0w
-    1:        CMP R0, R3, R0
-    2:        BEQ +(10)
-    3:        MOV R0, 1w
-    4:        SUB R2, R3, R0
-    5:        MUL R0, R3, R1
-    6:        STR R2, [0]
-    7:        STR R0, [1]
-    8:        LDR R1, [1]
-    9:        LDR R3, [0]
-   10:        BL -(10)
-   11:        BAL +(2)
-   12:        MOV R0, R1
-   13:        SWI 17
+    0:          mov     ip, sp
+    1:          stmfd   sp!, {fp,ip,lr,pc}
+    2:          sub     fp, ip, #1
+    3:          mov     r2, #0w
+    4:          cmp     r0, r2
+    5:          beq     + (8)
+    6:          mov     r2, #1w
+    7:          sub     r3, r0, r2
+    8:          mul     r2, r0, r1
+    9:          stmfd   sp!, {r3,r2}
+   10:          ldmfd   sp, {r0,r1}
+   11:          add     sp, sp, #2
+   12:          bal     - (9)
+   13:          mov     r0, r1
+   14:          sub     sp, fp, #2
+   15:          ldmfd   sp, {fp,sp,pc}
 Return:
-    R0 
+    r0
+
 *)
 
 
 (*
     val env6 = toANF [] f6_def;
     val arm6 = compileEnv env6;
-    val ARM6 = mk_ARM arm6;
 	
-	simT ARM6;
+    simR (mk_ARM arm6);
 
-val thm = fetch "-" "instB_def";
 
-val instB_thm = Q.prove
-(`(instB 0 =  ((MOV,NONE,F),SOME (REG 12),[REG 13],NONE)) /\
-  (instB 1 = ((STMFD,NONE,F),SOME (WREG 13), [REG 0; REG 2; REG 3; REG 11; REG 12; REG 14; REG 15],NONE)) /\
-  (instB 2 = ((SUB,NONE,F),SOME (REG 11),[REG 12; NCONST 1], NONE)) /\
-  (instB 3 = ((MOV,NONE,F),SOME (REG 2),[WCONST 0w],NONE)) /\
-  (instB 4 = ((CMP,NONE,F),NONE,[REG 0; REG 2],NONE)) /\
-  (instB 5 = ((B,SOME EQ,F),NONE,[REG 2],SOME (POS 8))) /\
-  (instB 6 = ((MOV,NONE,F),SOME (REG 2),[WCONST 1w],NONE)) /\
-  (instB 7 = ((SUB,NONE,F),SOME (REG 3), [REG 0; REG 2],NONE)) /\
-  (instB 8 = ((MUL,NONE,F),SOME (REG 2), [REG 0; REG 1],NONE)) /\
-  (instB 9 = ((STMFD,NONE,F),SOME (WREG 13), [REG 3; REG 2],NONE)) /\
-  (instB 10 = ((LDMFD,NONE,F),SOME (REG 13),[REG 0; REG 1],NONE)) /\
-  (instB 11 = ((ADD,NONE,F),SOME (REG 13),[REG 13; NCONST 2],NONE)) /\
-  (instB 12 = ((B,SOME AL,F),NONE,[],SOME (NEG 9))) /\
-  (instB 13 = ((MOV,NONE,F),SOME (REG 0),[REG 1],NONE)) /\
-  (instB 14 = ((SUB,NONE,F),SOME (REG 13),[REG 11; NCONST 5],NONE)) /\
-  (instB 15 = ((LDMFD,NONE,F),SOME (REG 13), [REG 0; REG 2; REG 3; REG 11; REG 13; REG 15],SOME INR))`
-,
- REPEAT CONJ_TAC THEN EVAL_TAC); 
+  REWRITE_TAC [read_thm] THEN
+  REPEAT STRIP_TAC THEN
+  
+  Induct_on `w2n (regs0 0)` THEN REPEAT STRIP_TAC THENL [
+	`regs0 0 = n2w 0` by METIS_TAC [w2n_ELIM] THEN
+	Q.PAT_ASSUM  `0 = i` (K ALL_TAC) THEN
+	IMP_RES_TAC (SPEC ``15`` TERRUN_THM) THEN
+  	ONCE_ASM_REWRITE_TAC [] THEN
+  	POP_ASSUM (K ALL_TAC)
+	(*
+	prove_arm [Once f6_def],	(* This would prove the basic case *)
+	*)
 
-  TAC0 [] THEN
-  Induct_on `w2n Ir3` THEN REPEAT STRIP_TAC THENL [
-	`Ir3 = 0w` by RW_TAC list_ss [w2n_ELIM] THEN
-	RW_TAC list_ss [Q.SPEC `15` TERRUN_THM] THEN
-	PAT_ASSUM ``0 = w2n Ir3`` (K ALL_TAC) THEN 
-	NTAC 6 TAC1 THEN
-	RW_TAC list_ss [TERRUN_STOP, Once f6_def],
+	IMP_RES_TAC WORD_IND_LEM THEN
+	IMP_RES_TAC (SPEC ``13`` TERRUN_THM) THEN
+        ONCE_ASM_REWRITE_TAC [] THEN
+        POP_ASSUM (K ALL_TAC) THEN
+	`?pc' cpsr' reg' mem'. (pc',cpsr',reg',mem') = run 13 (instB,16) (0,cpsr0,regs0,mems0)` 
+		by METIS_TAC [ABS_PAIR_THM] THEN
 
-	`(v = w2n (reg0 3 - 1w)) /\ ~(reg0 3 = 0w) /\ ~(reg0 3 < 0w)` by REWRITE_TAC [] THENL [
-		...
-		...
-	
-
-	RW_TAC list_ss [Q.SPEC `11` TERRUN_THM] THEN
-
-	`?pc' cpsr' reg' mem'. (pc',cpsr',reg',mem') = run 11 (instB,14) (0,cpsr0,reg0,mem0)` by ALL_TAC THENL [
-	    Q.ABBREV_TAC `s' = run 11 (instB,14) (0,cpsr0,reg0,mem0)` THEN
-	    `s' = (FST s', FST (SND s'), FST (SND (SND s')), SND (SND (SND s')))` by METIS_TAC [PAIR] THEN 
-	    METIS_TAC [],
-
-	`terminated (instB,14) (pc',cpsr',reg',mem') /\ 
-		(w2n (reg' 14) = 14) /\ (pc' = 0) /\ (reg' 3 = reg0 3 - 1w) /\ (reg' 1 = reg0 3 * reg0 1)` by ALL_TAC THENL [
+	`terminated (instB,16) (pc',cpsr',reg',mem') /\ 
+		((pc' = 3) /\ (reg' 3 = regs0 3 - 1w) /\ (reg' 1 = regs0 3 * regs0 1)` by 
+							ALL_TAC THENL [
 		STRIP_TAC THENL [
 			RW_TAC list_ss [TERMINATED_THM],
 			POP_ASSUM MP_TAC THEN
 			FULL_SIMP_TAC list_ss [WORD_ADD_SUB, w2n_11] THEN
-			NTAC 12 TAC1 THEN RW_TAC list_ss []
+			...			
+
+
 		]
 	
 		FULL_SIMP_TAC list_ss [w2n_11] THEN
